pulse/src/checker/Pulse.JoinComp.fst
@@ -22,6 +22,194 @@ open Pulse.Typing.Combinators
 open Pulse.Checker.Pure
 open Pulse.Checker.Base
 open Pulse.Checker.Prover
+open FStar.List.Tot
+open Pulse.Show
+module T = FStar.Tactics.V2
+module MKeys = Pulse.Checker.Prover.Match.MKeys
+module RT = FStar.Reflection.Typing
+module R = FStar.Reflection.V2
+module RU = Pulse.RuntimeUtils
+
+let may_match g (p:slprop) (q:slprop) = MKeys.eligible_for_smt_equality g p q
+
+let find_match g (p:slprop) (qs:list slprop)
+: T.Tac (list (slprop & slprop) & list slprop & list slprop)
+= let rec aux qs rest 
+  : T.Tac (list (slprop & slprop) & list slprop & list slprop)
+  = match qs with
+    | [] -> [], [p], rest
+    | q::qs ->
+      if may_match g p q 
+      then [p,q], [], qs@rest
+      else (
+        match inspect_term p, inspect_term q with
+        | Tm_Pure _, Tm_Pure _ -> [p,q], [], qs@rest
+        | _ -> aux qs (q::rest)
+      )
+  in
+  aux qs []
+
+let partition_matches g (ps qs:list slprop)
+: T.Tac (list (slprop & slprop) & list slprop & list slprop)
+= T.fold_right 
+    (fun p (matches, remaining_ps, remaining_qs) ->
+      let matches', remaining_ps', remaining_qs = find_match g p remaining_qs in
+      matches'@matches, remaining_ps'@remaining_ps, remaining_qs)
+    ps ([], [], qs)
+
+let rec combine_terms top g b pq : T.Tac term =
+  let p, q = pq in
+  T.print (
+    Printf.sprintf "Combine terms %s and %s\n" (show p) (show q)
+  );
+  let pack t = pack_term_view t (T.range_of_term p) in
+  let combine_terms p q = combine_terms true g b (p, q) in
+  let def () = if T.term_eq p q then p else RT.mk_if b p q in
+  match inspect_term p, inspect_term q with
+  | Tm_Emp, Tm_Emp
+  | Tm_SLProp, Tm_SLProp
+  | Tm_EmpInames, Tm_EmpInames
+  | Tm_Inames, Tm_Inames -> p
+  | Tm_Pure f1, Tm_Pure f2 ->
+    let f = RT.mk_if b f1 f2 in
+    pack <| Tm_Pure f
+  | Tm_Inv i1 p1, Tm_Inv i2 p2 ->
+    pack <| Tm_Inv (combine_terms i1 i2) (combine_terms p1 p2)
+  | Tm_FStar f1, Tm_FStar f2 -> (
+    if not top then def () else
+    let hd1, args1 = T.collect_app_ln f1 in
+    let hd2, args2 = T.collect_app_ln f2 in //not proving termination because collect_app_ln's type is not strong enough
+    T.print (
+      Printf.sprintf "Destructed\nlhs as %s [%s]\nrhs as %s [%s]"
+        (show hd1) (show args1)
+        (show hd2) (show args2)
+    );
+    if T.term_eq hd1 hd2
+    then T.mk_app hd1 (combine_args g b args1 args2)
+    else def ()
+  )
+  | _ -> def ()
+
+and combine_args g b (args1 args2:list R.argv) : T.Tac (list R.argv) =
+  //combinine args, when heads are equal, 
+  //the quals must be equal and the lengths must be equal
+  match args1, args2 with
+  | (a1, v1)::args1, (a2, v2)::args2 ->
+    (combine_terms true g b (a1, a2), v1)::combine_args g b args1 args2
+  | _ -> []
+
+let join_slprop g b (ex1 ex2:list (universe & binder)) (p1 p2:slprop)
+: T.Tac slprop
+= match inspect_term p1, inspect_term p2 with
+  | Tm_ExistsSL .., _
+  | Tm_ForallSL .., _
+  | _, Tm_ExistsSL ..
+  | _, Tm_ForallSL .. -> RT.mk_if b p1 p2
+    // let x1 = fresh g in
+    // let p1 = open_term_nv p1 (b1.binder_ppname, x1) in
+    // join_slprop g b ((u1, b1, p1)::ex1) ex2 p1 p2
+
+  // | _, Tm_ExistsSL u2 b2 p2 ->
+  //   let x2 = fresh g in
+  //   let p2 = open_term_nv p2 (b2.binder_ppname, x2) in
+  //   join_slprop g b ex1 ((u2, b2, p2)::ex2) p1 p2
+
+  | _ ->
+    let open Pulse.Show in
+    let p1s, p2s = slprop_as_list p1, slprop_as_list p2 in
+    let matches, p1s, p2s = partition_matches g p1s p2s in
+    T.print (
+      Printf.sprintf
+        "Matches: %s\nRemaining ps=%s\nRemaining qs=%s\n"
+          (show matches)
+          (show p1s)
+          (show p2s)
+    );
+    let matched = T.map (fun x -> combine_terms true g b x) matches in
+    match p1s, p2s with
+    | [], [] -> list_as_slprop matched
+    | _ ->
+      let remaining = RT.mk_if b (list_as_slprop p1s) (list_as_slprop p2s) in
+      list_as_slprop (remaining::matched)
+
+let rec join_effect_annot g (e1 e2:effect_annot)
+: T.Tac (e:effect_annot & effect_annot_typing g e)
+= match e1, e2 with
+  | _, EffectAnnotSTT
+  | EffectAnnotSTT, _ -> (| EffectAnnotSTT, () |)
+  
+  | EffectAnnotGhost { opens=o1 }, EffectAnnotGhost { opens=o2 } ->
+    let o = tm_join_inames o1 o2 in
+    let ty = Pulse.Checker.Pure.core_check_term g o RT.E_Total tm_inames in
+    let e = EffectAnnotGhost { opens = o } in
+    (| e, ty |)
+  | EffectAnnotAtomic { opens=o1 }, EffectAnnotAtomic { opens=o2 } ->
+    let o = tm_join_inames o1 o2 in
+    let ty = Pulse.Checker.Pure.core_check_term g o RT.E_Total tm_inames in
+    let e = EffectAnnotAtomic { opens = o } in
+    (| e, ty |)
+  | EffectAnnotAtomicOrGhost { opens=o1 }, EffectAnnotAtomicOrGhost { opens=o2 } ->
+    let o = tm_join_inames o1 o2 in
+    let ty = Pulse.Checker.Pure.core_check_term g o RT.E_Total tm_inames in
+    let e = EffectAnnotAtomicOrGhost { opens = o } in
+    (| e, ty |)
+
+  | EffectAnnotAtomicOrGhost { opens=o1 }, EffectAnnotGhost _ ->
+    join_effect_annot g (EffectAnnotGhost {opens=o1}) e2
+
+  | EffectAnnotAtomicOrGhost { opens=o1 }, EffectAnnotAtomic _ ->
+    join_effect_annot g (EffectAnnotAtomic {opens=o1}) e2
+
+  | EffectAnnotAtomic _, EffectAnnotAtomicOrGhost { opens=o2 } ->
+    join_effect_annot g e1 (EffectAnnotAtomicOrGhost {opens=o2})
+
+  | EffectAnnotGhost _, EffectAnnotAtomicOrGhost { opens=o2 } ->
+    join_effect_annot g e1 (EffectAnnotGhost {opens=o2})
+
+  | _ -> 
+    let open Pulse.PP in
+    let open Pulse.Show in
+    fail_doc g (Some <| range_of_env g)
+      [text "Could not combine effect annotations";
+       text (Printf.sprintf "Effect of then-branch is %s" (show e1));
+       text (Printf.sprintf "Effect of else-branch is %s" (show e2))]
+
+let join_post #g #hyp #b
+    (p1:post_hint_for_env (g_with_eq g hyp b tm_true))
+    (p2:post_hint_for_env (g_with_eq g hyp b tm_false))
+: T.Tac (post_hint_for_env g)
+= T.print (
+    Printf.sprintf "Joining postconditions:\n%s\nand\n%s\n"
+      (T.term_to_string p1.post)
+      (T.term_to_string p2.post)
+  );
+
+  if not (T.term_eq p1.ret_ty p2.ret_ty)
+  then (
+    fail_doc g (Some (T.range_of_term p1.ret_ty))
+      Pulse.PP.(
+        [text "The branches of a conditional must return the same type";
+         text (Printf.sprintf "The types %s and %s are not equal" (T.term_to_string p1.ret_ty) (T.term_to_string p2.ret_ty))]
+      )
+  );
+  let joined_post = join_slprop g b [] [] p1.post p2.post in
+  T.print (
+    Printf.sprintf "Inferred joint postcondition:\n%s\n"
+      (T.term_to_string joined_post)
+  );
+  let x = fresh g in
+  assume (fresh_wrt x g (freevars joined_post));
+  let (| u, ty_typing |) = Pulse.Checker.Pure.check_universe g p1.ret_ty in
+  let joined_post' = open_term_nv joined_post (ppname_default, x) in 
+  let g' = push_binding g x ppname_default p1.ret_ty in
+  let post_typing_src = Pulse.Checker.Pure.check_slprop_with_core g' joined_post' in
+  let (| eff, eff_ty |) = join_effect_annot g p1.effect_annot p2.effect_annot in
+  let res : post_hint_for_env g =
+    {g; effect_annot=eff; effect_annot_typing=eff_ty;
+     ret_ty=p1.ret_ty; u=u; ty_typing; x;
+     post=joined_post; post_typing_src; post_typing=RU.magic()}
+  in
+  res
 
 
 let st_ghost_as_atomic_matches_post_hint
