pulse/src/checker/Pulse.Checker.Abs.fst
@@ -318,7 +318,22 @@ let open_ascription (c:comp_ascription) (nv:nvar) : comp_ascription =
 let close_ascription (c:comp_ascription) (nv:nvar) : comp_ascription =
   subst_ascription c [RT.ND (snd nv) 0]
 
-#push-options "--z3rlimit_factor 8 --fuel 0 --ifuel 1 --split_queries no"
+let post_condition_to_be_inferred_hack var (post:term) : T.Tac (option term) =
+  match inspect_term post with
+  | Tm_FStar t -> (
+    match T.inspect_ln t with
+    | R.Tv_FVar fv -> (
+      if T.inspect_fv fv = ["TestBind"; "to_be_inferred"]
+      then None
+      else Some (open_term' post var 1) 
+    ) 
+    | _ -> Some (open_term' post var 1) 
+  ) 
+  | _ -> Some (open_term' post var 1)
+
+module R = FStar.Reflection.V2
+#push-options "--z3rlimit_factor 20 --fuel 0 --ifuel 1 --split_queries no --query_stats"
+#restart-solver
 let rec check_abs_core
   (g:env)
   (t:st_term{Tm_Abs? t.term})
@@ -412,7 +427,7 @@ let rec check_abs_core
           open_term_nv (comp_pre c) px,
           inames_opened,
           Some (open_term_nv (comp_res c) px),
-          Some (open_term' (comp_post c) var 1)
+          post_condition_to_be_inferred_hack var (comp_post c)
       in
       let (| pre_opened, pre_typing |) =
         (* In some cases F* can mess up the range in error reporting and make it
@@ -424,8 +439,7 @@ let rec check_abs_core
       let post : post_hint_opt g' =
         match post_hint_body with
         | None ->
-          let open Pulse.PP in
-          fail_doc g (Some body.range) [text "Top-level functions must be annotated with pre and post conditions"]
+          None
         | Some post ->
           let post_hint_typing
             : post_hint_t
@@ -440,6 +454,14 @@ let rec check_abs_core
 
       let ppname_ret = mk_ppname_no_range "_fret" in
       let r  = check g' pre_opened pre_typing post ppname_ret body_opened  in
+      let (| post, r |) : (ph:post_hint_opt g' & checker_result_t g' pre_opened ph) = 
+        match post with
+        | None -> 
+          let ph = Pulse.Checker.Base.infer_post r in
+          let r = Pulse.Checker.Prover.prove_post_hint r (Some ph) (T.range_of_term t) in
+          (| Some ph, r |)
+        | _ -> (| post, r |)
+      in
       let (| body, c_body, body_typing |) : st_typing_in_ctxt g' pre_opened post =
         apply_checker_result_k #_ #_ #(Some?.v post) r ppname_ret in
 
