pulse/src/checker/Pulse.Checker.Prover.RewritesTo.fst
@@ -22,6 +22,13 @@ module R = FStar.Reflection.V2
 
 let rewrites_to_p_lid = Pulse.Reflection.Util.mk_pulse_lib_core_lid "rewrites_to_p"
 
+let mk_sq_rewrites_to_p u t x y =
+  let open R in
+  let hd = pack_fv rewrites_to_p_lid in
+  let hd = pack_ln (Tv_UInst hd [u]) in
+  let args = [(t, Q_Implicit); (x, Q_Explicit); (y, Q_Explicit)] in
+  mk_squash u_zero (R.mk_app hd args)
+
 let extract_rewrites_to_p (t: typ) =
   let hd, args = R.collect_app_ln t in
   match R.inspect_ln hd, args with
